add some aggregator and primitive commands

QAL/AbstractHeap.v
@@ -1,10 +1,47 @@
 Require Import FSetInterface.
-Require Import Tactics  Algebra.SetoidCat  Algebra.Monad Algebra.SetoidCat.PairUtils Algebra.SetoidCat.MaybeUtils Algebra.Monad.Maybe Algebra.Alternative Algebra.Functor Algebra.FoldableFunctor Algebra.Applicative Algebra.Monoid Algebra.SetoidCat.NatUtils Algebra.SetoidCat.BoolUtils Algebra.Monoid.PropUtils.
+Require Import Tactics  Algebra.SetoidCat  Algebra.Monad Algebra.SetoidCat.PairUtils Algebra.SetoidCat.MaybeUtils Algebra.Monad.Maybe Algebra.Alternative Algebra.Functor Algebra.FoldableFunctor Algebra.Applicative Algebra.Monoid Algebra.SetoidCat.NatUtils Algebra.SetoidCat.BoolUtils Algebra.Monoid.PropUtils QAL.Definitions Algebra.SetoidCat.ListUtils Algebra.SetoidCat.UnitUtils.
 
 Require Import FMapWeakList  RelationClasses Relation_Definitions Morphisms SetoidClass.
 
+Inductive argument val :=
+| argumentVal : val -> argument val
+| argumentVar : var -> argument val
+.
 
-Module Type AbstractHeap.
+Definition argument_equiv val (valS : Setoid val) : relation (argument val) :=
+  fun a b => match a, b with
+               | argumentVal _ va, argumentVal _ vb => va == vb
+               | argumentVar _ va, argumentVar _ vb => va = vb
+               | _, _ => False
+             end
+.
+
+                                                           
+Instance argument_Equivalence val (valS : Setoid val) : Equivalence (argument_equiv val valS).
+Proof.
+  split.
+  - unfold Reflexive. intros. destruct x.
+    + simpl. reflexivity.
+    + simpl. auto.
+  - unfold Symmetric. intros. destruct x, y.        
+    + simpl in *. rewritesr.
+    + simpl in *. auto.
+    + simpl in *. auto.
+    + simpl in *. auto.
+  - unfold Transitive. intros. destruct x, y, z.
+    + simpl in *. rewritesr.
+    + simpl in *. auto.
+    + simpl in *. tauto. 
+    + simpl in *. auto.
+    + simpl in *. auto.
+    + simpl in *. tauto.
+    + simpl in *. auto.
+    + simpl in *. congruence.
+Qed.
+
+Program Instance argumentS val (valS : Setoid val) : Setoid (argument val).
+
+Module Type AbstractHeap (PT : PredType) (VT : ValType).
   Parameter t : Type.
   Parameter tS : Setoid t.
   Parameter l : forall A, (Setoid A) -> Type.
@@ -17,6 +54,9 @@ Module Type AbstractHeap.
   Parameter isEmpty : tS ~> iff_setoid.
   Parameter disjoint : tS ~> tS ~~> iff_setoid.
   Parameter union : tS ~> tS ~~> tS.
+  Parameter lookup : PT.predS ~> listS (argumentS _ VT.valS) ~~> tS ~~> lS _ (listS (varS ~*~ VT.valS)).
+  Parameter insert : PT.predS ~> listS VT.valS ~~> tS ~~> maybeS tS.
+  Parameter delete : PT.predS ~> listS VT.valS ~~> tS ~~> maybeS tS.
 
   Notation "a ⊥ b" := (disjoint @ a @ b) (at level 15). 
   Notation "a ⋅ b" := (union @ a @ b) (at level 15). 
